

<section>
  <title>Derivatives of the Exponential and Logarithmic Functions</title>
  <p>
    We know how to take the derivative of <m>f(x) = x^2,</m> but what about <m>g(x) = 2^x</m> or <m>h(x) = e^x?</m> We wish to be able to differentiate exponential and logarithmic functions. If you need a review of these functions, then work through <xref ref="appexp">Appendix</xref>.
    EXTRA<fn>Even as I appreciate the logic and value of early transcendental texts, I strongly prefer teaching the integral definition for the natural log and deriving the properties of the natural log function and the exponential functions from there.  Still, we teach early transcendental functions and this is the most elegant way I know of to define <m>e</m> under that constraint. As always, I present this slowly and interactively urging questions as I go in an attempt to maximize understanding.</fn></p>

  <problem>
    <statement>
      <p>
        Sketch graphs of <m>f(x) = 2^x</m> and <m>g(x) = 3^x</m> on the same coordinate axes labeling several points and being very careful to show which function is above the other at various points on the graph.
      </p>
    </statement>
  </problem>

  <example>
    <statement>
      <p>
        Defining <m>e</m> and finding the derivative of the function <m>e^x</m>.
      </p>
    </statement>
  </example>

  <p>
    Consider finding the derivative of <m>f(x) = 2^x.</m> Using limits to compute the derivative, we have:
    <md>
      <mrow>f'(x) \amp  = \amp  \lim_{h \rightarrow 0} \frac{f(x+h)-f(x)}{h}  \;\;\;
      \mbox{by definition of derivative}</mrow>
      <mrow>\amp  = \amp  \lim_{h \rightarrow 0} \frac{2^{x+h}-2^x}{h} \;\;\;  \mbox{by definition of}  \; \; f</mrow>
      <mrow>\amp  = \amp   \lim_{h \rightarrow 0} \frac{2^x(2^h-1)}{h} \;\;\; \mbox{by algebra}</mrow>
      <mrow>\amp  = \amp   \lim_{h \rightarrow 0} 2^x\frac{2^h-1}{h} \;\;\;   \mbox{by algebra}</mrow>
      <mrow>\amp  = \amp   2^x \lim_{h \rightarrow 0} \frac{2^h-1}{h} \;\;\;  \mbox{by the \textit{Constant Multiple Rule for limits}}</mrow>
      <mrow>\amp  = \amp   2^x f'(0)</mrow>
    </md>
  </p>

  <p>
    We would now know the derivative of the function <m>2^x</m> if only we could determine <m>f'(0) = \dsp{\lim_{h \rightarrow 0} \frac{2^{h}-1}{h}}.</m> We can approximate <m>f'(0) = \dsp{\lim_{h \rightarrow 0} \frac{2^{h}-1}{h}} \approx .69</m> by using a limit table. Similarly, if we went through the same process for <m>g(x) = 3^x</m> we would see that <m>g'(0) = \dsp{\lim_{h \rightarrow 0} \frac{3^{h}-1}{h}} \approx 1.09</m> by using a limit table. Since the slope of <m>f</m> at 0 is less than 1 and the slope of <m>g</m> at 0 is greater than one, it makes sense that there should be an exponential function which has slope <em>exactly</em> 1 at 0. We define a number, called <m>e</m>, to be the number (between 2 and 3) so that <m>\dsp{\lim_{h \rightarrow 0} \frac{e^{h}-1}{h}} = 1.</m> Now, if we let <m>j(x) = e^x</m> then we have
    <md>
      <mrow>j'(x) \amp  = \amp  \lim_{h \rightarrow 0} \frac{j(x+h)-j(x)}{h}  \;\;\;
      \mbox{by definition of derivative}</mrow>
      <mrow>\amp  = \amp  \lim_{h \rightarrow 0} \frac{e^{x+h}-e^x}{h} \;\;\;  \mbox{by definition of}  \; \; f</mrow>
      <mrow>\amp  = \amp   \lim_{h \rightarrow 0} \frac{e^x(e^h-1)}{h} \;\;\; \mbox{by algebra}</mrow>
      <mrow>\amp  = \amp   \lim_{h \rightarrow 0} e^x\frac{e^h-1}{h} \;\;\;   \mbox{by algebra}</mrow>
      <mrow>\amp  = \amp   e^x \lim_{h \rightarrow 0} \frac{e^h-1}{h} \;\;\;  \mbox{by the \textit{Constant Multiple Rule for limits}}</mrow>
      <mrow>\amp  = \amp   e^x f'(0)</mrow>
      <mrow>\amp =\amp  e^x.</mrow>
    </md>
  </p>

  <p>
    This work results in a definition and a theorem.
  </p>

  <definition>
    <statement>
      <p>
        Let <m>e</m> be the number that satisfies <m>\dsp \lim_{h \to 0} \frac{e^h-1}{h} = 1</m>.
      </p>
    </statement>
  </definition>

  <theorem>
    <statement>
      <p>
        <em>Exponential Derivative Theorem.</em> If <m>f(x) = e^x</m>, then <m>f'(x) = e^x</m>.
      </p>
    </statement>
  </theorem>

  <definition>
    <statement>
      <p>
        Let <m>g(x)=\ln(x)</m> be the function that is the inverse of the function <m>f(x) = e^x</m>.
      </p>
    </statement>
  </definition>

  <p>
    <em>Algebra Reminders</em>
    <ol>
      <li>
        <p>
          <m>f(x)=e^x</m> has domain all <m>x \in \re</m> and range all <m>x > 0</m>
        </p>
      </li>

      <li>
        <p>
          <m>g(x)=\ln(x)</m> has domain all <m>x > 0</m> and range all <m>x \in \re</m>
        </p>
      </li>

      <li>
        <p>
          <m>e^{x+y} = e^x e^y</m> and <m>{(e^x)}^{^y} = e^{xy}</m> for all <m>x,y \in \re</m>
        </p>
      </li>

      <li>
        <p>
          <m>\ln(xy) = \ln(x) + \ln(y)</m>  for all <m>x>0</m>, <m>y>0</m>
        </p>
      </li>

      <li>
        <p>
          <m>\ln(x^y) = y\ln(x)</m> for all <m>y \in \re</m> and <m>x>0</m>
        </p>
      </li>

      <li>
        <p>
          <m>e^{\ln(x)} = x</m> for all <m>x > 0</m>
        </p>
      </li>

      <li>
        <p>
          <m>\ln(e^x)=x</m> for all <m>x \in \re</m>
        </p>
      </li>

      <li>
        <p>
          <m>\log_b(x) = \ln(x)/ln(b)</m> for all <m>b \in \re</m> (except <m>b</m>=1) and for all <m>x>0</m>
        </p>
      </li>
    </ol>
  </p>

  <problem>
    <statement>
      <p>
        Compute and simplify the derivatives of the following functions:
        <ol>
          <li>
            <p>
              <m>g(x) = e^x  + x^2  +  2x</m>
            </p>
          </li>

          <li>
            <p>
              <m>f(x) = xe^x</m>
            </p>
          </li>

          <li>
            <p>
              <m>h(x) = x^3/e^x</m>
            </p>
          </li>

          <li>
            <p>
              <m>f(x) = e^{x^2}</m>
            </p>
          </li>

          <li>
            <p>
              <m>f(x) = 3x^2e^{x^4}</m>
            </p>
          </li>
        </ol>
      </p>
    </statement>
  </problem>

  <problem>
    <statement>
      <p>
        Let <m>g(x) = \ln(x)</m>. Here are two clever ways to compute the derivative of <m>g</m>; do which ever you like better!
        <ol>
          <li>
            <p>
              Since we know that <m>g(e^x)=x,</m> differentiate both sides of this equation using the Chain Rule and then solve for <m>g'(x).</m>
            </p>
          </li>

          <li>
            <p>
              Apply the exponential function to both sides of the equations <m>g(x)=\ln(x)</m>, differentiate, and then solve for <m>g'(x).</m>
            </p>
          </li>
        </ol>
      </p>
    </statement>
  </problem>

  <problem>
    <statement>
      <p>
        Compute and simplify the derivative of the following functions:
        <ol>
          <li>
            <p>
              <m>g(x) = \ln(7x-8)</m>
            </p>
          </li>

          <li>
            <p>
              <m>f(x) = x^2\ln(x)</m>
            </p>
          </li>

          <li>
            <p>
              <m>h(x) = x^3/\ln(3x^2 - x^{1/3})</m>
            </p>
          </li>
        </ol>
      </p>
    </statement>
  </problem>

  <problem xml:id="logdiff">
    <statement>
      <p>
        Let <m>h(x) = 2^x</m> and compute <m>h'</m> first by taking the natural log of both sides and then taking the derivative of both sides.
      </p>
    </statement>
  </problem>

  <problem>
    <statement>
      <p>
        Compute and simplify the derivative of the following functions:
        <ol>
          <li>
            <p>
              <m>g(x) = 2^{7x-8}</m>
            </p>
          </li>

          <li>
            <p>
              <m>f(x) = 2^x - x^2</m>
            </p>
          </li>

          <li>
            <p>
              <m>h(x) = 3^{x^2}</m>
            </p>
          </li>
        </ol>
      </p>
    </statement>
  </problem>

  <problem>
    <statement>
      <p>
        Use the change-of-base formula, <m>\log_b(x) = \ln(x)/\ln(b)</m>, to compute the derivative of <m>L(x) = \log_3(x^5-2x).</m>
      </p>
    </statement>
  </problem>
</section>

